I noticed a bad little bug in the definition of AlgebraicTable: It didn’t specify that the default value for the table HT was default. Which led to such bad type inference that the inferred types for BranchTableAlgebraic were not general at all, and the provided proof was completely specialized to this. I fixed the bug in AlgebraicTable and replaced the proof of BranchTableAlgebraic with a correct, general one. Also, I simplified the type specifications throughout and defined FunBranchTable.

BranchTable.v
@@ -84,7 +84,7 @@ Class Table (key V:Type) (default:V) `{EqDec key} :=
     set : key -> V -> table -> table;
   }.
 
-Class AlgebraicTable (key V:Type) (default:V) `(Table key V) :=
+Class AlgebraicTable {key V:Type} {default:V} `(HT:Table key V default) :=
   {
     get_empty_default : forall (k : key), get k empty = default;
     get_set_same : forall (k : key) (v : V) (t : table),
@@ -102,14 +102,14 @@ Class AlgebraicTable (key V:Type) (default:V) `(Table key V) :=
   }.
 
 #[export] Instance FunTableAlgebraic (key V:Type) (default:V) `{EqDec key} :
-  @AlgebraicTable key V default _ _ _ (FunTable key V default).
+  AlgebraicTable (FunTable key V default).
 Proof.
   constructor; auto; intros; simpl.
   - destruct (eqb_eq k k) as [_ Heq]. rewrite Heq; auto.
   - destruct (eqb_neq k k') as [Hneq _]. rewrite Hneq; auto.
 Qed.
 
-#[export] Instance BranchTable (key1 key2 V : Type) (default:V)
+#[export] Instance BranchTable {key1 key2 V : Type} {default:V}
   `(HT2 : Table key2 V default) `(HT1 : Table key1 HT2.(table) HT2.(empty))
   : Table (prod key1 key2) V default :=
   {
@@ -123,26 +123,37 @@ Qed.
                  end
   }.
 
-#[export] Instance BranchTableAlgebraic (key1 key2 V : Type) (default:V)
-  `{HT2 : Table key2 V default} `{HT1 : Table key1 HT2.(table) HT2.(empty)}
-  `{HAT2 : AlgebraicTable key2 V default}
-  `{HAT1 : AlgebraicTable key1 HT2.(table) HT2.(empty)} :
-  AlgebraicTable (prod key1 key2) V default (BranchTable key1 key2 V default _ _).
+#[export] Instance BranchTableAlgebraic {key1 key2 V : Type} {default:V}
+  `(HT2 : Table key2 V default) `(HT1 : Table key1 HT2.(table) HT2.(empty))
+  `{HAT2 : @AlgebraicTable key2 V default _ _ HT2}
+  `{HAT1 : @AlgebraicTable key1 HT2.(table) HT2.(empty) _ _ HT1} :
+  @AlgebraicTable (prod key1 key2) V default _ _ (BranchTable HT2 HT1).
 Proof.
-  constructor; intros; destruct k as [k1 k2]; auto.
-  - simpl.
-    destruct (eqb_eq k1 k1) as [_ Heq1]. rewrite Heq1; auto.
-    destruct (eqb_eq k2 k2) as [_ Heq2]. rewrite Heq2; auto.
-  - destruct k' as [k1' k2']. simpl.
-    destruct (eqb_reflect k1 k1') as [?|?],
-        (eqb_reflect k2 k2') as [?|?]; subst; auto.
-    + exfalso. auto.
+  constructor; intros; destruct k as [k1 k2]; simpl.
+  - rewrite HAT1.(get_empty_default), HAT2.(get_empty_default). auto.
+  - rewrite HAT1.(get_set_same), HAT2.(get_set_same). auto.
+  - destruct k' as [k1' k2'].
+    destruct (eqb_reflect k1 k1') as [?|?]; subst.
+    + rewrite HAT1.(get_set_same).
+      destruct (eqb_reflect k2 k2') as [?|?]; subst.
+      * exfalso. auto.
+      * rewrite HAT2.(get_set_other); auto.
+    + rewrite HAT1.(get_set_other); auto.
 Qed.
 
-Definition natnatboolBranchTable := (BranchTable nat nat bool false (FunTable _ _ _) (FunTable _ _ _)).
+Definition natnatboolBranchTable := (BranchTable (FunTable nat bool false) (FunTable nat _ _)).
+Definition natnatboolBranchTableAlgebraic : AlgebraicTable natnatboolBranchTable := BranchTableAlgebraic _ _.
 
-Definition natnatboolBranchTableAlgebraic : AlgebraicTable _ _ _ natnatboolBranchTable := BranchTableAlgebraic _ _ _ _.
+Definition FunBranchTable (key1:Type) `{EqDec key1} {key2 V:Type} {default:V}
+  `(HT2 : Table key2 V default) := (BranchTable HT2 (FunTable _ _ _)).
 
-Check natnatboolBranchTable.
+Definition FunBranchTableAlgebraic {key1 key2 V: Type} {default:V} `{EqDec key1}
+  `(HT2 : Table key2 V default) `{HAT2 : @AlgebraicTable key2 V default _ _ HT2} :
+  AlgebraicTable (FunBranchTable key1 HT2) := BranchTableAlgebraic _ _.
 
-Compute natnatboolBranchTable.(get) (1,3) (natnatboolBranchTable.(set) (1,2) true natnatboolBranchTable.(empty)).
+Example natnatboolBranchTable' := FunBranchTable nat (FunTable nat bool false).
+Example natnatnatboolBranchTable' := FunBranchTable nat (FunBranchTable nat (FunTable nat bool false)).
+Example natnatnatnatboolBranchTable' := FunBranchTable nat (FunBranchTable nat (FunBranchTable nat (FunTable nat bool false))).
+Example natnatnatnatnatboolBranchTable' := FunBranchTable nat (FunBranchTable nat (FunBranchTable nat (FunBranchTable nat (FunTable nat bool false)))).
+
+Compute natnatboolBranchTable'.(get) (1,3) (natnatboolBranchTable'.(set) (1,2) true natnatboolBranchTable'.(empty)).
